@prefix : <https://nfdi4culture.de/ontology#> .
@prefix dc: <http://purl.org/dc/elements/1.1/> .
@prefix mo: <http://purl.org/ontology/mo/> .
@prefix cto: <https://nfdi4culture.de/ontology#> .
@prefix n4c: <https://nfdi4culture.de/id/> .
@prefix owl: <http://www.w3.org/2002/07/owl#> .
@prefix rdf: <http://www.w3.org/1999/02/22-rdf-syntax-ns#> .
@prefix xml: <http://www.w3.org/XML/1998/namespace> .
@prefix xsd: <http://www.w3.org/2001/XMLSchema#> .
@prefix rdfs: <http://www.w3.org/2000/01/rdf-schema#> .
@prefix schema: <http://schema.org/> .
@prefix dcterms: <http://purl.org/dc/terms/> .
@prefix nfdicore: <https://nfdi.fiz-karlsruhe.de/ontology/> .
@base <https://nfdi4culture.de/ontology#> .

<https://nfdi4culture.de/ontology#> rdf:type owl:Ontology ;
                                     dc:creator n4c:E1925 ,
                                                n4c:E2415 ,
                                                n4c:E2416 ,
                                                n4c:E3095 ;
                                     dc:title "NFDI4Culture Ontology" ;
                                     dcterms:abstract """The NFDI4Culture ontology (CTO) is an ontology for the representation and categorization of various resources within the domain of NFDI4Culture. It encompasses a wide array of entities including datasets, individual items and cultural heritage objects, data providers, persons, projects, and other pertinent elements relevant to cultural heritage and research endeavors. CTO is a module that builds upon the NFDIcore Ontology (https://ise-fizkarlsruhe.github.io/nfdicore/). With the advent of version v.2.2.0, CTO is aligned with NFDIcore v.2.0.0 and its subsequent versions, while ensuring compatibility with the Basic Formal Ontology (BFO).

At its core, the ontology provides a structured means to describe and connect diverse entities, facilitating efficient organization, retrieval, and analysis of cultural data. By defining classes such as cto:DatafeedElement, cto:Item, it establishes clear distinctions and relationships between different types of resources, enabling nuanced classification and enhanced comprehension of the domain.

Moreover, the ontology incorporates essential properties and relationships, such as cto:elementOf, nfdicore:publisher, nfdicore:license, and cto:temporalCoverage, to enrich the descriptions of resources and provide additional contextual information and intrconnection of elements across culture disciplines. This ensures a more robust representation of cultural artifacts, datasets, and associated metadata, thereby supporting a wide range of scholarly and practical applications within the NFDI4Culture ecosystem."""@en ;
                                     dcterms:bibliographicCitation "Oleksandra Bruns, Tabea Tietz, Etienne Posthumus, Harald Sack. NFDI4Culture Ontology. Revision: v2.2.0. Retrieved from:"^^rdfs:Literal ;
                                     dcterms:hasVersion "v2.2.0"^^rdfs:Literal ;
                                     <http://purl.org/vocab/vann/preferredNamespacePrefix> "cto"^^rdfs:Literal ;
                                     <http://purl.org/vocab/vann/preferredNamespaceUri> <https://creativecommons.org/publicdomain/zero/1.0/> ,
                                                                                        <https://nfdi4culture.de/ontology#> ;
                                     rdfs:label "NFDI4Culture Ontology (cto)" ;
                                     rdfs:seeAlso <https://nfdi4culture.de/ontology.json> ,
                                                  <https://nfdi4culture.de/ontology.nt> ,
                                                  <https://nfdi4culture.de/ontology.rdf> ,
                                                  <https://nfdi4culture.de/ontology.ttl> ,
                                                  <https://nfdi4culture.de/ontology/about.html> ;
                                     owl:priorVersion "2.1"^^rdfs:Literal ;
                                     owl:versionInfo "v.2.2.0" .

#################################################################
#    Annotation properties
#################################################################

###  http://purl.org/dc/elements/1.1/creator
dc:creator rdf:type owl:AnnotationProperty .


###  http://purl.org/dc/elements/1.1/title
dc:title rdf:type owl:AnnotationProperty .


###  http://purl.org/dc/terms/abstract
dcterms:abstract rdf:type owl:AnnotationProperty .


###  http://purl.org/dc/terms/bibliographicCitation
dcterms:bibliographicCitation rdf:type owl:AnnotationProperty .


###  http://purl.org/dc/terms/hasVersion
dcterms:hasVersion rdf:type owl:AnnotationProperty .


###  http://purl.org/dc/terms/license
dcterms:license rdf:type owl:AnnotationProperty .


###  http://purl.org/vocab/vann/preferredNamespacePrefix
<http://purl.org/vocab/vann/preferredNamespacePrefix> rdf:type owl:AnnotationProperty .


###  http://purl.org/vocab/vann/preferredNamespaceUri
<http://purl.org/vocab/vann/preferredNamespaceUri> rdf:type owl:AnnotationProperty .


###  https://nfdi.fiz-karlsruhe.de/ontology/example
nfdicore:example rdf:type owl:AnnotationProperty .


#################################################################
#    Datatypes
#################################################################

###  http://www.w3.org/2001/XMLSchema#date
xsd:date rdf:type rdfs:Datatype .


#################################################################
#    Object Properties
#################################################################

###  http://purl.org/dc/terms/isPartOf
dcterms:isPartOf rdf:type owl:ObjectProperty ;
                 owl:equivalentProperty schema:isPartOf ;
                 rdfs:domain nfdicore:Resource ;
                 rdfs:range nfdicore:Resource ;
                 rdfs:comment "This property establishes a connection between a resource and the overarching resource to which it belongs, e.g. an individual item to the dataset it is part of."@en .


###  http://purl.org/ontology/mo/lyrics
mo:lyrics rdf:type owl:ObjectProperty ;
          rdfs:domain mo:MusicalWork ;
          rdfs:range mo:Lyrics ;
          rdfs:comment "This property establishes a connection between a resource of type musical work and a lyrics entity."@en .


###  http://schema.org/image
schema:image rdf:type owl:ObjectProperty ;
             rdfs:domain cto:DatafeedElement ;
             rdfs:range owl:Thing .


###  http://schema.org/isPartOf
schema:isPartOf rdf:type owl:ObjectProperty .


###  http://schema.org/url
schema:url rdf:type owl:ObjectProperty .


###  https://nfdi4culture.de/ontology#aat
cto:aat rdf:type owl:ObjectProperty ;
        rdfs:subPropertyOf cto:externalVocabulary ;
        rdfs:domain schema:CreativeWork ;
        rdfs:range owl:Thing ;
        rdfs:comment "The property relates a creative work resource to a concept, term, or classification type in Art & Architecture Thesaurus."@en ;
        rdfs:label "AAT"@en ;
        nfdicore:example "A stained glass window artwork \"Engel mit Dudelsack\" has a related AAT entry <http://vocab.getty.edu/page/aat/300263722>"@en .


###  https://nfdi4culture.de/ontology#ddbAPI
cto:ddbAPI rdf:type owl:ObjectProperty ;
           rdfs:subPropertyOf schema:url ;
           rdfs:domain nfdicore:Resource ;
           rdfs:range owl:Thing ;
           rdfs:comment "The property relates the resource to the DDB API Endpoint associated with the resource."@en ;
           rdfs:label "DDB API"^^rdfs:Literal ;
           nfdicore:example "https://api.deutsche-digitale-bibliothek.de/items/OUOATUXI6I7XMWYRRKAXGXGEM3E6JD3D/source/record"^^rdfs:Literal .


###  https://nfdi4culture.de/ontology#elementOf
cto:elementOf rdf:type owl:ObjectProperty ;
              rdfs:subPropertyOf dcterms:isPartOf ;
              rdfs:domain cto:DatafeedElement ;
              rdfs:range nfdicore:Resource ;
              rdfs:comment "This property connects an element and the overarching resource it belongs to, e.g. an individual item and the dataset it is part of."@en ;
              rdfs:label "element of"@en ;
              nfdicore:example "\"Engel mit Dudelsack\" is a single element in the digital image dataset Corpus Vitrearum Medii Aevi Deutschland"@en .


###  https://nfdi4culture.de/ontology#elementType
cto:elementType rdf:type owl:ObjectProperty ;
                rdfs:domain cto:DatafeedElement ;
                rdfs:range owl:Thing ;
                rdfs:comment """The property is recommended to be used in combination with the subproperties of cto:externalVocabulary to specify the vocabulary the element type is defined with:

For example:
<:Frühlingsgruß   cto:elementType <https://rism.online/subjects/25227>>
<:Frühlingsgruß   cto:rism <https://rism.online/subjects/25227>>"""@en ,
                             "The property relates a datafeed element to its category within a predefined vocabulary/taxonomy, indicating the nature or genre of the element. The type must be taken from a published controlled vocabulary, e.g. AAT, GND, Wikidata, Iconclass, FactGrid, etc."@en ;
                rdfs:label "element type"@en ;
                nfdicore:example """http://vocab.getty.edu/aat/300003725 (altars (religious fixtures))
http://vocab.getty.edu/aat/300047090 (sculpture (visual works))
https://www.wikidata.org/wiki/Q101687 (altar)"""^^rdfs:Literal .


###  https://nfdi4culture.de/ontology#externalVocabulary
cto:externalVocabulary rdf:type owl:ObjectProperty ;
                       rdfs:domain owl:Thing ;
                       rdfs:range owl:Thing ;
                       rdfs:comment """The property and its subproperties are recommended to be used in combination with:

cto:elementType
cto:subjectConcept
cto:relatedPerson
cto:relatedLocation

For example:
<:Frühlingsgruß   cto:rism <https://rism.online/subjects/25227>>
<:Frühlingsgruß   cto:elementType <https://rism.online/subjects/25227>>"""@en ,
                                    "This property establishes a connection between a thing and an external controlled vocabulary, providing additional semantic information from external sources. The subproperties of cto:externalVocabulary should be used for standard reference systems such as AAT, GeoNames, GND, Iconclass, Wikidata, RISM."@en ;
                       rdfs:label "external vocabulary"@en .


###  https://nfdi4culture.de/ontology#factgrid
cto:factgrid rdf:type owl:ObjectProperty ;
             rdfs:subPropertyOf cto:externalVocabulary ;
             rdfs:domain owl:Thing ;
             rdfs:range owl:Thing ;
             rdfs:comment "Adolph Freiherr Knigge has element type \"Human\" (<https://database.factgrid.de/wiki/Item:Q7>) in FactGrid database."@en ,
                          "The property relates a thing to a concept, term, or classification type in FactGrid database."@en ;
             rdfs:label "FactGrid"@en .


###  https://nfdi4culture.de/ontology#geonames
cto:geonames rdf:type owl:ObjectProperty ;
             rdfs:subPropertyOf cto:externalVocabulary ;
             rdfs:domain owl:Thing ;
             rdfs:range owl:Thing ;
             rdfs:comment "The property relates a thing to a location in the GeoNames geographical database."@en ;
             rdfs:label "GeoNames"@en ;
             nfdicore:example "A stained glass window artwork \"Engel mit Dudelsack\" has a related GeoNames location <http://sws.geonames.org/11427995>"@en .


###  https://nfdi4culture.de/ontology#gnd
cto:gnd rdf:type owl:ObjectProperty ;
        rdfs:subPropertyOf cto:externalVocabulary ;
        rdfs:domain owl:Thing ;
        rdfs:range owl:Thing ;
        rdfs:comment "The property relates a thing to the corresponding entry or related concept of the thing in GND (Integrated Authority File)."@en ;
        rdfs:label "GND"@en ;
        nfdicore:example "A caricature image \"Gedichte eines Kleinstädters\" has a related GND entry <https://d-nb.info/gnd/118680609>"@en .


###  https://nfdi4culture.de/ontology#iconclass
cto:iconclass rdf:type owl:ObjectProperty ;
              rdfs:subPropertyOf cto:externalVocabulary ;
              rdfs:domain schema:CreativeWork ;
              rdfs:range owl:Thing ;
              rdfs:comment "The property relates a creative work to the subject concept or content of the creative work in the Iconclass classification system."@en ;
              rdfs:label "Iconclass"@en ;
              nfdicore:example "A stained glass window artwork \"Engel mit Dudelsack\" has a related Iconclass entry <https://iconclass.org/11G21>"@en .


###  https://nfdi4culture.de/ontology#iiifImageAPI
cto:iiifImageAPI rdf:type owl:ObjectProperty ;
                 rdfs:subPropertyOf schema:url ;
                 rdfs:domain cto:DatafeedElement ;
                 rdfs:range owl:Thing ;
                 rdfs:comment "The property relates the datafeed element to the IIIF Image API associated with the image of the element."@en ;
                 rdfs:label "IIIF Image API"^^rdfs:Literal ;
                 nfdicore:example "https://heidicon.ub.uni-heidelberg.de/iiif/2/2305%3A2123"^^rdfs:Literal .


###  https://nfdi4culture.de/ontology#iiifPresentationAPI
cto:iiifPresentationAPI rdf:type owl:ObjectProperty ;
                        rdfs:subPropertyOf schema:url ;
                        rdfs:domain cto:DatafeedElement ;
                        rdfs:range owl:Thing ;
                        rdfs:comment "The property relates the datafeed element to the IIIF Presentation API associated with the element."@en ;
                        rdfs:label "IIIF Presentation API"^^rdfs:Literal ;
                        nfdicore:example "https://heidicon.ub.uni-heidelberg.de/iiif/2/597256:51961/info.json"@en .


###  https://nfdi4culture.de/ontology#incipitOf
cto:incipitOf rdf:type owl:ObjectProperty ;
              rdfs:subPropertyOf dcterms:isPartOf ;
              rdfs:domain cto:Incipit ;
              rdfs:range schema:MusicComposition ;
              rdfs:comment "The property connects an incipit and the music composition it belongs to."@en ;
              rdfs:label "incipit of"@en ;
              nfdicore:example "https://rism.online/sources/201001959/incipits/1.1.1 is an incipit of musical composition \"Frühlingsgruß\" (https://rism.online/sources/201001959) by Robert Schumann."@en .


###  https://nfdi4culture.de/ontology#oai-pmhAPI
cto:oai-pmhAPI rdf:type owl:ObjectProperty ;
               rdfs:subPropertyOf schema:url ;
               rdfs:domain nfdicore:Resource ;
               rdfs:range owl:Thing ;
               rdfs:comment "The property relates the resource to the OAI-PMH API Endpoint associated with the resource."@en ;
               rdfs:label "OAI-PMH API"^^rdfs:Literal ;
               nfdicore:example "https://heidicon.ub.uni-heidelberg.de/api/v1/plugin/base/oai/oai?verb=GetRecord&metadataPrefix=lido&identifier=oai:heidicon.ub.uni-heidelberg.de:ed84679c-e602-4b7c-9e77-f8b5c9c97b74"^^rdfs:Literal .


###  https://nfdi4culture.de/ontology#relatedEvent
cto:relatedEvent rdf:type owl:ObjectProperty ;
                 rdfs:domain cto:DatafeedElement ;
                 rdfs:range nfdicore:Event ;
                 rdfs:comment "The property establishes a connection between an element and the diverse events associated with the described datafeed element, which may include attendance, hosting, performance, sponsorship, or collaboration, contributing, witnessing, etc. of a specific event."@en ,
                              """The property is recommended to be used in combination with the subproperties of cto:externalVocabulary to explicitly indicate the vocabulary through which the event related to the element is defined:

For example:
<:AdolphFreiherrKnigge cto:relatedEvent <https://database.factgrid.de/entity/Q23430>>
<:AdolphFreiherrKnigge cto:factgrid <https://database.factgrid.de/entity/Q23430>>"""@en ;
                 rdfs:label "related event"@en .


###  https://nfdi4culture.de/ontology#relatedItem
cto:relatedItem rdf:type owl:ObjectProperty ;
                rdfs:domain cto:DatafeedElement ;
                rdfs:range cto:Item ;
                rdfs:comment """The property is recommended to be used in combination with the subproperties of cto:externalVocabulary to explicitly indicate the vocabulary through which the item related to the element is defined:

For example:
<:AdolphFreiherrKnigge cto:relatedItem <https://database.factgrid.de/entity/Q12913>>
<:AdolphFreiherrKnigge cto:factgrid <https://database.factgrid.de/entity/Q12913>>"""@en ,
                             "The property relates a datafeed element to an item it is related to."@en ;
                rdfs:label "related item"@en .


###  https://nfdi4culture.de/ontology#relatedLocation
cto:relatedLocation rdf:type owl:ObjectProperty ;
                    rdfs:domain cto:DatafeedElement ;
                    rdfs:range nfdicore:Place ;
                    rdfs:comment """The property establishes a connection between an element and the locations that are associated with the described datafeed element. These locations may include the physical location of the item, the geographical setting depicted in the item, the locations explicitly mentioned or implied within the item's content, the birth or death places of a person, the location of an event, etc. The locations must be taken from a published controlled vocabulary, e.g. GND, Wikidata, GeoNames.

In contrast to nfdicore:location, it covers broader aspects of locations associated with an element, including physical, geographical, and content-related locations. Additionally, it enforces the use of a controlled vocabulary for specifying these locations."""@en ,
                                 """The property is recommended to be used in combination with the subproperties of cto:externalVocabulary to specify the vocabulary the location related to the element is defined with:

For example:
<:EngelMitDudelsack   cto:relatedLocation <http://sws.geonames.org/11427995>>
<:EngelMitDudelsack   cto:geonames <http://sws.geonames.org/11427995>>"""@en ;
                    rdfs:label "related location"@en ;
                    nfdicore:example """https://sws.geonames.org/2950159/ (Berlin)
https://www.wikidata.org/wiki/Q64 (Berlin)"""^^rdfs:Literal .


###  https://nfdi4culture.de/ontology#relatedOrganization
cto:relatedOrganization rdf:type owl:ObjectProperty ;
                        rdfs:domain cto:DatafeedElement ;
                        rdfs:range nfdicore:Organization ;
                        rdfs:comment """The property is recommended to be used in combination with the subproperties of cto:externalVocabulary to explicitly indicate the vocabulary through which the organization related to the element is defined:

For example:
<:AdolphFreiherrKnigge cto:relatedOrganization <https://database.factgrid.de/entity/Q81288>>
<:AdolphFreiherrKnigge cto:factgrid <https://database.factgrid.de/entity/Q81288>>"""@en ,
                                     "The property links an element to the various organizations affiliated with the described datafeed element. These organizations encompass a diverse range, such as educational institutions, workplaces, interest groups, event organizers, etc. The organizations must be taken from a published controlled vocabulary, e.g. GND, Wikidata, FactGrid."@en ;
                        rdfs:label "related organization"@en .


###  https://nfdi4culture.de/ontology#relatedPerson
cto:relatedPerson rdf:type owl:ObjectProperty ;
                  rdfs:domain cto:DatafeedElement ;
                  rdfs:range nfdicore:Person ;
                  rdfs:comment """The property is recommended to be used in combination with the subproperties of cto:externalVocabulary to explicitly indicate the vocabulary through which the person related to the datafeed element is defined:

For example:
<:WasIhrWollt cto:relatedPerson <http://www.wikidata.org/entity/Q692>>
<:WasIhrWollt cto:wikidata <http://www.wikidata.org/entity/Q692>>"""@en ,
                               "The property relates an element to individuals associated with the described element. These individuals may include item creators, set/costume designers, actors, addressers, performers, relatives, friends, event participants, etc. The individuals must be taken from a published controlled vocabulary, e.g. GND, Wikidata."@en ;
                  rdfs:label "related person"@en ;
                  nfdicore:example """https://www.wikidata.org/wiki/Q34628 (Gotthold Ephraim Lessing)
https://d-nb.info/gnd/142585777 (Wilke, Insa)"""@en .


###  https://nfdi4culture.de/ontology#rism
cto:rism rdf:type owl:ObjectProperty ;
         rdfs:subPropertyOf cto:externalVocabulary ;
         rdfs:domain mo:MusicalWork ;
         rdfs:range owl:Thing ;
         rdfs:comment "The property relates a musical item to the corresponding entry or related concept of the item in RISM (Répertoire International des Sources Musicales)."@en ;
         rdfs:label "RISM"@en ;
         nfdicore:example "A musical composition \"Frühlingsgruß\" has a related RISM entry <https://rism.online/subjects/25227>"@en .


###  https://nfdi4culture.de/ontology#sourceFile
cto:sourceFile rdf:type owl:ObjectProperty ;
               rdfs:subPropertyOf schema:url ;
               rdfs:domain nfdicore:Resource ;
               rdfs:range owl:Thing ;
               rdfs:comment "The property links a resource to the URL of a data source from which it originates, e.g. in an API endpoint."@en ;
               rdfs:label "source file"^^rdfs:Literal ;
               nfdicore:example "https://heidicon.ub.uni-heidelberg.de/api/v1/plugin/base/oai/oai?verb=GetRecord&metadataPrefix=lido&identifier=oai:heidicon.ub.uni-heidelberg.de:ed84679c-e602-4b7c-9e77-f8b5c9c97b74"^^rdfs:Literal .


###  https://nfdi4culture.de/ontology#subjectConcept
cto:subjectConcept rdf:type owl:ObjectProperty ;
                   rdfs:domain cto:DatafeedElement ;
                   rdfs:range owl:Thing ;
                   rdfs:comment """The property is recommended to be used in combination with the subproperties of cto:externalVocabulary to specify the vocabulary the subject concept is defined with:

For example:
<:EngelMitDudelsack   cto:subjectConcept <https://iconclass.org/11G21>>
<:EngelMitDudelsack   cto:iconclass <https://iconclass.org/11G21>>"""@en ,
                                "The property relates an element to concepts related to the subject of the element within a predefined vocabulary/taxonomy. It may be used to associate the item with specific ideas, themes, or topics, e.g. iconography, themes from literature, terms, concepts, related works that item is based on, domain of interest of a person, theme of the event, etc. The subject must be taken from a published controlled vocabulary, e.g. AAT, GND, Wikidata, Iconclass."@en ;
                   rdfs:label "subject concept"@en ;
                   nfdicore:example """http://iconclass.org/11H (saints)
https://iconclass.org/11K (devil(s) and demons)
https://www.wikidata.org/wiki/Q581450 (fallen angel)
https://d-nb.info/gnd/4099291-3 (Minna von Barnhelm)"""@en .


###  https://nfdi4culture.de/ontology#viaf
cto:viaf rdf:type owl:ObjectProperty ;
         rdfs:subPropertyOf cto:externalVocabulary ;
         rdfs:domain owl:Thing ;
         rdfs:range owl:Thing ;
         rdfs:comment "The property relates a thing to the corresponding entry in VIAF: Virtual International Authority File."@en ;
         rdfs:label "VIAF"@en ;
         nfdicore:example "Robert Schumann has a corresponding VIAF entity <https://viaf.org/viaf/7575259>"@en .


###  https://nfdi4culture.de/ontology#wikidata
cto:wikidata rdf:type owl:ObjectProperty ;
             rdfs:subPropertyOf cto:externalVocabulary ;
             rdfs:domain owl:Thing ;
             rdfs:range owl:Thing ;
             rdfs:comment "The property relates a thing to the corresponding entry or related concept of the item in Wikidata."@en ;
             rdfs:label "Wikidata"@en ;
             nfdicore:example "A theatrical performance of \"Was ihr Wollt\" has a related Wikidata entry <http://www.wikidata.org/entity/Q221211>"@en .


#################################################################
#    Data properties
#################################################################

###  http://purl.org/ontology/mo/text
mo:text rdf:type owl:DatatypeProperty ;
        rdfs:domain mo:Lyrics ;
        rdfs:range rdfs:Literal ;
        rdfs:comment "The property relates the lyrics entity of a musical work and its text." .


###  http://schema.org/temporalCoverage
schema:temporalCoverage rdf:type owl:DatatypeProperty ;
                        rdfs:comment "The generic property that relates an item to its broad temporal attributes, e.g. the period of its existence, the dates of the creation, destruction, and approximate dates."@en ,
                                     "Use related properties e.g. nfdcore:birthDate, nfdicore:deathDate for describing Persons, or nfdicore:startDate, nfdicore:endDate for describing Events."@en .


###  https://nfdi4culture.de/ontology#approximatePeriod
cto:approximatePeriod rdf:type owl:DatatypeProperty ;
                      rdfs:subPropertyOf schema:temporalCoverage ;
                      rdfs:domain cto:Item ;
                      rdfs:range rdfs:Literal ;
                      rdfs:comment "The property relates an item to the approximate time the item is associated with. It often links to time periods/dates containing temporal constraints, e.g. \"during, before, after\" to approximate the time. The property should only be used to express an estimated or imprecise date associated with an item when the exact date is uncertain or not precisely known."@en ;
                      rdfs:label "approximate period"@en ;
                      nfdicore:example "\"vor 1397\", \"nach 15 Jahrhundert\""^^rdfs:Literal .


###  https://nfdi4culture.de/ontology#clef
cto:clef rdf:type owl:DatatypeProperty ;
         rdfs:domain cto:Incipit ;
         rdfs:range rdfs:Literal ;
         rdfs:comment "A clef is a symbol at the beginning of a musical piece that indicates the pitch of the written notes."@en ,
                      "The property relates an incipit to its clef."@en ;
         rdfs:label "clef"@en ;
         nfdicore:example "\"G-2\"" .


###  https://nfdi4culture.de/ontology#creationDate
cto:creationDate rdf:type owl:DatatypeProperty ;
                 rdfs:subPropertyOf schema:temporalCoverage ;
                 rdfs:domain cto:Item ;
                 rdfs:range [ rdf:type rdfs:Datatype ;
                              owl:unionOf ( xsd:date
                                            xsd:dateTime
                                            xsd:dateTimeStamp
                                          )
                            ] ;
                 rdfs:comment "The property relates an item to the exact date when the item was created or came into existence."@en ;
                 rdfs:label "creation date"@en ;
                 nfdicore:example "\"1380-01-01T00:00:00\""^^rdfs:Literal .


###  https://nfdi4culture.de/ontology#creationPeriod
cto:creationPeriod rdf:type owl:DatatypeProperty ;
                   rdfs:subPropertyOf schema:temporalCoverage ;
                   rdfs:domain cto:Item ;
                   rdfs:range rdfs:Literal ;
                   rdfs:comment "The property links an item to the time period that indicates the time span during which the item was created."@en ;
                   rdfs:label "creation period"@en ;
                   nfdicore:example "\\\"1888\\\", \\\"1380-01-01T00:00:00/1400-12-31T23:59:59\\\", \\\"18-19 Jh\\\""@en .


###  https://nfdi4culture.de/ontology#destructionDate
cto:destructionDate rdf:type owl:DatatypeProperty ;
                    rdfs:subPropertyOf schema:temporalCoverage ;
                    rdfs:domain cto:Item ;
                    rdfs:range [ rdf:type rdfs:Datatype ;
                                 owl:unionOf ( xsd:date
                                               xsd:dateTime
                                               xsd:dateTimeStamp
                                             )
                               ] ;
                    rdfs:comment "The property relates an item to the specific date on which the item ceases to exist or is intentionally terminated, discarded, or removed."@en ;
                    rdfs:label "destruction date"@en ;
                    nfdicore:example "\"1891-07-06T00:00:00\""^^rdfs:Literal .


###  https://nfdi4culture.de/ontology#elementTypeLiteral
cto:elementTypeLiteral rdf:type owl:DatatypeProperty ;
                       rdfs:domain cto:DatafeedElement ;
                       rdfs:range rdfs:Literal ;
                       rdfs:comment "The property relates a datafeed element to its broader category, indicating the nature of the element."@en ,
                                    "cto:elementTypeLiteral should only be used when associated item types lack URIs or when the use of cto:elementType is not possible."@en ;
                       rdfs:label "element type literal"@en ;
                       nfdicore:example "\"Glaskunst (Objektgattung)\", \"Schauspiel\", \"Fliegende Blätter\", \"Human\""^^rdfs:Literal .


###  https://nfdi4culture.de/ontology#relatedEventLiteral
cto:relatedEventLiteral rdf:type owl:DatatypeProperty ;
                 rdfs:domain cto:DatafeedElement ;
                 rdfs:range rdfs:Literal ;
                 rdfs:comment "The property relates an element to events related to the element in a textual or non-URI-based representation."@en ,
                              "cto:relatedEventLiteral should only be used when associated organizations lack URIs or when the use of cto:relatedEvent is not possible."@en ;
                 rdfs:label "related event literal"@en .


###  https://nfdi4culture.de/ontology#existencePeriod
cto:existencePeriod rdf:type owl:DatatypeProperty ;
                    rdfs:subPropertyOf schema:temporalCoverage ;
                    rdfs:domain cto:Item ;
                    rdfs:range rdfs:Literal ;
                    rdfs:comment "The property links an item to the time period that indicates the time span during which the item existed. The property should only be used when the use of cto:creationDate and cto:distructionDate is not possible."@en ;
                    rdfs:label "existence period"@en ;
                    nfdicore:example "\"17 Jahrhundert\", \"1890s\""@en .


###  https://nfdi4culture.de/ontology#keySignature
cto:keySignature rdf:type owl:DatatypeProperty ;
                 rdfs:domain cto:Incipit ;
                 rdfs:range rdfs:Literal ;
                 rdfs:comment "A key signature is a set of sharp or flat symbols placed on the staff at the beginning of a piece of music, indicating the key of the composition."@en ,
                              "The property relates an incipit to its key signature."@en ;
                 rdfs:label "key signature"@en ;
                 nfdicore:example "\"xF\""^^rdfs:Literal .


###  https://nfdi4culture.de/ontology#relatedLocationLiteral
cto:relatedLocationLiteral rdf:type owl:DatatypeProperty ;
                    rdfs:domain cto:DatafeedElement ;
                    rdfs:range rdfs:Literal ;
                    rdfs:comment "The property relates a datafeed element to locations associated with the described element in a textual or non-URI-based representation."@en ,
                                 "cto:relatedLocationLiteral should only be used when associated locations lack URIs or when the use of cto:relatedLocation is not possible."@en ;
                    rdfs:label "related location literal"@en ;
                    nfdicore:example "\"Abtei Altenberg\", \"Berlin\""^^rdfs:Literal .


###  https://nfdi4culture.de/ontology#relatedOrganizationLiteral
cto:relatedOrganizationLiteral rdf:type owl:DatatypeProperty ;
                        rdfs:domain cto:DatafeedElement ;
                        rdfs:range rdfs:Literal ;
                        rdfs:comment "The property relates an element to organizations related to the element in a textual or non-URI-based representation."@en ,
                                     "cto:relatedOrganizationLiteral should only be used when associated organizations lack URIs or when the use of cto:relatedOrganization is not possible."@en ;
                        rdfs:label "related organization literal"@en .


###  https://nfdi4culture.de/ontology#pattern
cto:pattern rdf:type owl:DatatypeProperty ;
            rdfs:domain cto:Incipit ;
            rdfs:range rdfs:Literal ;
            rdfs:comment "A pattern of an incipit refers to an initial sequence of notes, chords, or rhythms."@en ,
                         "The property relates an incipit to its pattern."@en ;
            rdfs:label "pattern"@en ;
            nfdicore:example "\"4'D/8.6GB4AG/8.6''EC2'A/4.''D8'BAG/4BA\""^^rdfs:Literal .


###  https://nfdi4culture.de/ontology#relatedPersonLiteral
cto:relatedPersonLiteral rdf:type owl:DatatypeProperty ;
                  rdfs:domain cto:DatafeedElement ;
                  rdfs:range rdfs:Literal ;
                  rdfs:comment "The property relates a datafeed element to individuals associated with the described element in a textual or non-URI-based representation."@en ,
                               "cto:relatedPersonLiteral should only be used when associated persons lack URIs or when the use of cto:relatedPerson is not possible."@en ;
                  rdfs:label "related person literal"@en ;
                  nfdicore:example "\"Felix Cziossek\""^^rdfs:Literal .


###  https://nfdi4culture.de/ontology#subjectConceptLiteral
cto:subjectConceptLiteral rdf:type owl:DatatypeProperty ;
                          rdfs:domain cto:DatafeedElement ;
                          rdfs:range rdfs:Literal ;
                          rdfs:comment "The property relates an element to concepts related to the subject of the element in a textual or non-URI-based representation."@en ,
                                       "cto:subjectConceptLiteral should only be used when associated concepts lack URIs or when the use of cto:subjectConcept is not possible."@en ;
                          rdfs:label "subject concept literal"@en ;
                          nfdicore:example "\"Coro\", \"Monumente\""^^rdfs:Literal .


###  https://nfdi4culture.de/ontology#timeSignature
cto:timeSignature rdf:type owl:DatatypeProperty ;
                  rdfs:domain cto:Incipit ;
                  rdfs:range rdfs:Literal ;
                  rdfs:comment "A time signature is a notation convention that indicates the number of beats in each measure and which note value represents one beat."@en ,
                               "The property relates an incipit to its time signature."@en ;
                  rdfs:label "time signature"@en ;
                  nfdicore:example "\"3/4\", \"4/4\""^^rdfs:Literal .


#################################################################
#    Classes
#################################################################

###  http://purl.org/ontology/mo/Lyrics
mo:Lyrics rdf:type owl:Class .


###  http://purl.org/ontology/mo/MusicalWork
mo:MusicalWork rdf:type owl:Class ;
               owl:equivalentClass schema:MusicComposition .


###  http://schema.org/CreativeWork
schema:CreativeWork rdf:type owl:Class ;
                    owl:equivalentClass cto:Item .


###  http://schema.org/MediaObject
schema:MediaObject rdf:type owl:Class ;
                   rdfs:subClassOf schema:CreativeWork .


###  http://schema.org/MusicComposition
schema:MusicComposition rdf:type owl:Class ;
                        rdfs:subClassOf schema:CreativeWork .


###  https://nfdi.fiz-karlsruhe.de/ontology/Event
nfdicore:Event rdf:type owl:Class .


###  https://nfdi.fiz-karlsruhe.de/ontology/Organization
nfdicore:Organization rdf:type owl:Class .


###  https://nfdi.fiz-karlsruhe.de/ontology/Person
nfdicore:Person rdf:type owl:Class .


###  https://nfdi.fiz-karlsruhe.de/ontology/Place
nfdicore:Place rdf:type owl:Class .


###  https://nfdi.fiz-karlsruhe.de/ontology/Resource
nfdicore:Resource rdf:type owl:Class .


###  https://nfdi4culture.de/ontology#DatafeedElement
cto:DatafeedElement rdf:type owl:Class ;
                    rdfs:subClassOf nfdicore:Resource ;
                    rdfs:comment "A datafeed element refers to an individual data point or entry within a larger dataset."@en ,
                                 "Datafeed element"@en ,
                                 """DatafeedElement serves to signify membership within a particular resource or datafeed. Thus, entities of various types—such as of types nfdicore:Person, nfdicore:Place, cto:Item, or nfdicore:Event, etc. may acquire the additional designation of DatafeedElement if they are included in e.g. a dataset and are described within the graph.

The recommended properties to describe datafeed elements: 

cto:elementOf
nfdicore:publisher
nfdicore:license
schema:url
cto:elementType
cto:subjectConcept
cto:relatedPerson
cto:relatedItem
cto:relatedEvent
cto:relatedOrganisation
cto:relatedLocation
cto:externalVocabulary
schema:temporalCoverage"""@en .


###  https://nfdi4culture.de/ontology#Incipit
cto:Incipit rdf:type owl:Class ;
            rdfs:subClassOf schema:CreativeWork ;
            rdfs:comment "A resource that represents an opening segment of a music composition."@en ;
            rdfs:label "Incipit"@en ;
            nfdicore:example "https://rism.online/sources/201001959/incipits/1.1.1"@en .


###  https://nfdi4culture.de/ontology#Item
cto:Item rdf:type owl:Class ;
         rdfs:comment "A creative work that represents a discrete, identifiable item within diverse resources, e.g. individual artwork in a collection, a record in a dataset, etc."@en ,
                      "item is a subclass of \\\"schema:CreativeWork\\\", indicating that all items inherently fall under the umbrella of creative works. However, for more refined classification, one can employ more specific subclasses of \\\"schema:CreativeWork,\\\" such as \\\"schema:VisualArtwork,\\\" \\\"schema:Photograph,\\\" or \\\"schema:MusicComposition,\\\" to better define the RDF type of an item and achieve a more granular level of categorization."@en ;
         rdfs:label "Item"@en ;
         nfdicore:example "A photograph of the stone sword Matū Ajimā Mandira, a single theatrical performance of \"Was ihr Wollt\" staged on March 11, 1923, a musical composition \"Frühlingsgruß\", a stained glass window artwork \"Engel mit Dudelsack\", a page from a satirical magazine featuring a poem and a caricature image titled \"Gedichte eines Kleinstädters\" ."@en .


###  Generated by the OWL API (version 4.5.9.2019-02-01T07:24:44Z) https://github.com/owlcs/owlapi
